src/Assembly/WithBedrock/SymbolicProofs.v
@@ -526,21 +526,41 @@ Ltac step_SetFlag :=
     [eassumption|..|clear H]
   end.
 
+(* ----------------------------------------------*)
+(* GETTING OPERATIONS *)
+(* ----------------------------------------------*)
 
-(* symbolic state s machine state m, related *)
-(* if calling GetReg on register r in state s is gives idx i and updates to state s', then *)
-(* s' is still related to m AND s is subsumed in s' AND eval i in s' gives us the original value of r in the machine state *)
+Lemma GetRegFull_R s m (HR : R s m) rn i s'
+  (H : GetRegFull rn s = Success (i, s'))
+  : s' = s /\ exists v,
+      eval s i v /\
+      Tuple.nth_default 0 (N.to_nat rn) (m : reg_state) = v.
+Proof using Type.
+  cbv [GetRegFull some_or] in H.
+  destruct (Symbolic.get_reg _ _) eqn:Hg in H; inversion_ErrorT; Prod.inversion_prod; subst.
+  split; [reflexivity|].
+  destruct s', m; eapply get_reg_R_regs; [apply HR | exact Hg].
+Qed.
+
+Ltac step_GetRegFull :=
+  match goal with
+  | H : Symbolic.GetRegFull ?rn ?s = Success (?i, ?s') |- _ =>
+      let Heq := fresh "Heq" s' in
+      let v := fresh "v" in let Hv := fresh "H" v in let Hnth := fresh "Hnth" in
+      case (GetRegFull_R s _ ltac:(eassumption) _ _ _ H) as (Heq & v & Hv & Hnth);
+      clear H;
+      subst s'
+  end.
+
 Lemma GetReg_R {opts : symbolic_options_computed_opt} {descr:description} s m (HR: R s m) r i s'
   (H : GetReg r s = Success (i, s'))
   : R s' m  /\ s :< s' /\ eval s' i (get_reg m r).
 Proof using Type.
-  cbv [GetReg GetRegFull bind some_or get_reg index_and_shift_and_bitcount_of_reg] in *.
-  pose proof (get_reg_R s _ ltac:(eassumption) (reg_index r)) as Hr.
-  destruct Symbolic.get_reg in *; [|inversion H]; cbn in H.
-  specialize (Hr _ eq_refl); case Hr as (v&Hi0&Hv).
-  rewrite Hv; clear Hv.
-  step_symex; eauto.
-  repeat (eauto || econstructor); cbn [interp_op].
+  cbv [GetReg get_reg index_and_shift_and_bitcount_of_reg] in *.
+  step_symex; step_GetRegFull; cbv [fst snd] in *. 
+  step_App. repeat (eauto || econstructor); cbn [interp_op].
+  split; [exact Hs'|split; [exact Hls'|]].
+  rewrite Hnth. exact Hi.
 Qed.
 
 Ltac step_GetReg :=
@@ -551,37 +571,6 @@ Ltac step_GetReg :=
     unshelve (edestruct t as (Hs'&Hlt&Hv); clear H); shelve_unifiable;
     [eassumption|..|clear H]
   end.
-
-Lemma mapM_fold_left_R {A} {opts : symbolic_options_computed_opt} {descr : description}
-  (f_sym : A -> M unit)
-  (f_sem : machine_state -> A -> machine_state)
-  (Hstep : forall a s m s',
-    R s m -> f_sym a s = Success (tt, s') ->
-    R s' (f_sem m a) /\ s :< s')
-  : forall l s m s',
-    R s m ->
-    Symbolic.mapM_ f_sym l s = Success (tt, s') ->
-    R s' (fold_left f_sem l m) /\ s :< s'.
-Proof using Type.
-Admitted.
-  (* induction l as [|a l IH]; intros s0 m0 s_final HR0 Hsym.
-  - cbv [Symbolic.mapM_ Symbolic.mapM] in Hsym.
-    rewrite Symbolic.unfold_bind in Hsym.
-    cbv [Symbolic.ret] in Hsym.
-    inversion Hsym; subst. split; [exact HR0 | apply subsumed_refl].
-  - cbn [fold_left].
-    cbv [Symbolic.mapM_] in Hsym.
-    cbn [Symbolic.mapM] in Hsym.
-    rewrite !Symbolic.unfold_bind in Hsym.
-    destruct (f_sym a s0) as [[? s1]|] eqn:Hstep_a; [|inversion Hsym].
-    destruct (Symbolic.mapM f_sym l s1) as [[? s2]|] eqn:Hrest; [|inversion Hsym].
-    cbv [Symbolic.ret] in Hsym. inversion Hsym; subst.
-    destruct (Hstep a s0 m0 s1 HR0 Hstep_a) as [HR1 Hsub1].
-    assert (Hsym' : Symbolic.mapM_ f_sym l s1 = Success (tt, s_final)).
-    { cbv [Symbolic.mapM_]. rewrite Symbolic.unfold_bind. rewrite Hrest. cbv [Symbolic.ret]. reflexivity. }
-    destruct (IH s1 (f_sem m0 a) s_final HR1 Hsym') as [HR_final Hsub_final].
-    split; [exact HR_final | eauto using subsumed_trans].
-  Qed. *)
 
 Lemma Address_R {opts : symbolic_options_computed_opt} {descr:description} s m (HR : R s m) (sa:AddressSize) o a s' (H : Symbolic.Address o s = Success (a, s'))
   : R s' m /\ s :< s' /\ exists v, eval s' a v /\ @DenoteAddress sa m o = v.
@@ -716,6 +705,25 @@ Proof.
   apply option_all_app.
 Qed.
 
+Lemma option_all_split {A} (l1 l2 : list (option A)) r :
+  option_all (l1 ++ l2) = Some r ->
+  exists r1 r2, option_all l1 = Some r1
+             /\ option_all l2 = Some r2
+             /\ r = r1 ++ r2.
+Proof.
+  revert r. induction l1 as [|x l1 IH]; intros r H; cbn in *.
+  - exists nil, r. eauto.
+  - destruct x; [|discriminate].
+    destruct (option_all (l1 ++ l2)) as [ys|] eqn:Eapp; [|discriminate].
+    injection H; clear H; intro; subst r.
+    specialize (IH _ eq_refl).
+    destruct IH as (r1 & r2 & H1 & H2 & ->).
+    exists (a :: r1), r2.
+    rewrite H1.
+    split; [reflexivity | split; [exact H2 | reflexivity]].
+Qed.
+
+
 Lemma get_mem_addr_mod (m : mem_state) a n :
     get_mem m (Z.land a (Z.ones 64)) n = get_mem m a n.
 Proof.
@@ -724,10 +732,102 @@ Proof.
   exact (word_of_Z_land_ones_64 a).
 Qed.
 
-Lemma SetMem_addr_mod m addr n v :                                                            
-  SetMem m (Z.land addr (Z.ones 64)) n v = SetMem m addr n v.
-Proof. 
-  cbv [SetMem Crypto.Util.Option.bind set_mem]. rewrite word_of_Z_land_ones_64. reflexivity. 
+Lemma mod_pow2_add_low (a c : Z) (k : nat) :
+  0 <= a < 2^8 ->
+  (a + c * 2^8) mod 2^(8 + 8 * Z.of_nat k) =
+  a + (c mod 2^(8 * Z.of_nat k)) * 2^8.
+Proof.
+  intros Ha.
+  rewrite Z.pow_add_r by lia.
+  rewrite Z.mul_comm with (n := 2^8) (m := 2^(8 * Z.of_nat k)).
+  (* now goal is (a + c * 2^8) mod (2^(8*k) * 2^8) = a + c mod 2^(8*k) * 2^8 *)
+  apply (Z.mod_small a (2^8)) in Ha.
+  assert (H8 : 0 < 2 ^ 8) by (apply Z.pow_pos_nonneg; lia).
+  assert (Hk : 0 < 2 ^ (8 * Z.of_nat k)) by (apply Z.pow_pos_nonneg; lia).
+  pose proof (Z.mod_pos_bound a (2 ^ 8) H8) as [Ha1 Ha2].
+  rewrite Ha in Ha1, Ha2.
+  pose proof (Z.mod_pos_bound c (2 ^ (8 * Z.of_nat k)) Hk) as [Hc1 Hc2].
+  rewrite (Z_div_mod_eq_full c (2 ^ (8 * Z.of_nat k))) at 1.
+  replace ((2 ^ (8 * Z.of_nat k) * (c / 2 ^ (8 * Z.of_nat k)) +
+            c mod 2 ^ (8 * Z.of_nat k)) * 2 ^ 8)
+    with (c mod 2 ^ (8 * Z.of_nat k) * 2 ^ 8 +
+          c / 2 ^ (8 * Z.of_nat k) * (2 ^ (8 * Z.of_nat k) * 2 ^ 8))
+    by ring.
+  rewrite Z.add_assoc, Z_mod_plus_full.
+  apply Z.mod_small. nia.
+Qed.
+
+Lemma le_combine_cons_add b bs :
+  le_combine (b :: bs) = Byte.byte.unsigned b + le_combine bs * 2^8.
+Proof.
+  replace (b :: bs) with ([b] ++ bs) by reflexivity.
+  rewrite (le_combine_app [b] bs).
+  rewrite le_combine_1.
+  cbn [length].
+  rewrite Z.shiftl_mul_pow2 by lia.
+  change (Z.of_nat 1 * 8) with 8.
+  apply bitblast.Z.or_to_plus.
+  pose proof Byte.byte.unsigned_range b.
+  apply Z.bits_inj_iff'; intros i Hi.
+  rewrite Z.land_spec, Z.bits_0.
+  destruct (Z.ltb_spec i 8).
+  - replace (le_combine bs * 2^8) with (Z.shiftl (le_combine bs) 8)
+      by (rewrite Z.shiftl_mul_pow2 by lia; reflexivity).
+    rewrite Z.shiftl_spec_low by lia.
+    apply Bool.andb_false_r.
+  - destruct (Z.eq_dec (Byte.byte.unsigned b) 0) as [Hz|Hnz].
+    + rewrite Hz, Z.bits_0. reflexivity.
+    + rewrite (Z.bits_above_log2 (Byte.byte.unsigned b) i).
+      lia.
+      lia.
+      apply Z.log2_lt_pow2. lia.
+      eapply Z.lt_le_trans; [exact (proj2 H)|].
+      apply Z.pow_le_mono_r; lia.
+Qed.
+
+Lemma le_combine_firstn n bs :
+  (n <= length bs)%nat ->
+  le_combine (firstn n bs) = Z.land (le_combine bs) (Z.ones (8 * Z.of_nat n)).
+Proof.
+  revert bs; induction n as [|n IH]; intros [|b bs] Hn; cbn [firstn length] in *.
+  - reflexivity (* both sides 0 *).
+  - simpl le_combine; rewrite Z.land_0_r; reflexivity.
+  - lia.
+  - rewrite !le_combine_cons_add.
+    rewrite IH by lia.
+    rewrite !Z.land_ones by lia.
+    pose proof Byte.byte.unsigned_range b.
+    replace (8 * Z.of_nat (S n)) with (8 + 8 * Z.of_nat n) by lia.
+    symmetry; apply mod_pow2_add_low; assumption.
+Qed.
+
+
+Lemma load_bytes_truncate (m : mem_state) a n1 n2 bs :
+  load_bytes m (word.of_Z a) (n1 + n2) = Some bs ->
+  load_bytes m (word.of_Z a) n1 = Some (firstn n1 bs).
+Proof.
+  unfold load_bytes. rewrite footprint_app, List.map_app.
+  intro H.
+  apply option_all_split in H.
+  destruct H as (r1 & r2 & H1 & H2 & ->).
+  rewrite H1. f_equal.
+  pose proof (length_load_bytes m (word.of_Z a) n1 r1) as Hlen.
+  unfold load_bytes in Hlen. specialize (Hlen H1).
+  rewrite firstn_app, Hlen, Nat.sub_diag, firstn_O, app_nil_r.
+  rewrite firstn_all2 by lia. reflexivity.
+Qed.
+
+Lemma get_mem_truncate m a n1 n2 v :
+  get_mem m a (n1 + n2) = Some v ->
+  get_mem m a n1 = Some (Z.land v (Z.ones (8 * Z.of_nat n1))).
+Proof.
+  cbv [get_mem Crypto.Util.Option.bind]. intros H.
+  destruct (load_bytes m (word.of_Z a) (n1 + n2)) as [bs|] eqn:Eall;
+    [|discriminate].
+  injection H; clear H; intro; subst v.
+  pose proof (length_load_bytes _ _ _ _ Eall) as Hlen.
+  apply load_bytes_truncate in Eall. rewrite Eall. f_equal.
+  apply le_combine_firstn. lia.
 Qed.
 
 (* if reading [chunks*8] bytes from va is v1,
@@ -738,10 +838,6 @@ Lemma get_mem_app_split m va (chunks : nat) v1 v2 :
   get_mem m (Z.land (va + Z.of_nat (8*chunks)) (Z.ones 64)) 8 = Some v2 ->
   get_mem m va (8*chunks + 8) = Some (Z.lor v1 (Z.shiftl v2 (64 * Z.of_nat chunks))).
 Proof.
-  (** 
-  |         v1        | v2 |
-  |----|----|----|----|----|
-  *)
   intros H1 H2.
   cbv [get_mem Crypto.Util.Option.bind] in *.
   (* unpack Hget m va (8*chunks) = Some v1 *)
@@ -767,6 +863,7 @@ Proof.
   rewrite word_of_Z_land_ones_64.
   symmetry. apply word.ring_morph_add.  
 Qed.
+
 
 (* General (n*64)-bit load. Load128_R / Load256_R are corollaries below. *)
 Lemma LoadN_R {opts : symbolic_options_computed_opt} {descr:description} 
@@ -875,6 +972,88 @@ Proof using Type.
   eapply LoadN_R with (n := 4%nat) in H; eauto.
 Qed.
 
+Lemma Load_R {opts : symbolic_options_computed_opt} {descr:description}
+  {sz : OperationSize} {sa : AddressSize} (Hsa : sa = 64%N)
+  s m (HR : R s m) a i s'
+  (H : Symbolic.Load a s = Success (i, s'))
+  : R s' m /\ s :< s' /\
+    exists v,
+      eval s' i v /\
+      get_mem m (DenoteAddress sa m a) (N.to_nat (operand_size a sz / 8)) = Some v.
+Proof.
+  cbv [Load] in H.
+  step_symex; cbv [fst snd] in *.
+  step_Address.
+  repeat (destruct_one_match_hyp; try discriminate H).
+  step_symex.
+  { (* 8 and 64 bit cases*) 
+    eapply (Load64_R s0 m) in HSv as (Hs1 & v0 & Heval_ & Hget_mem & Hv0_bd); eauto. subst s1.
+    step_App; repeat (econstructor; eauto).
+    destruct E as [E|E]; rewrite E in *.
+    { (* 8 bit *)
+      rewrite H3. change 8%nat with (1 + 7)%nat in Hget_mem.
+      apply get_mem_truncate in Hget_mem.
+      change (N.to_nat (8 / 8)) with 1%nat.
+      rewrite Hget_mem. reflexivity.
+    }
+    { (* 64 bit *) 
+      rewrite H3. replace (N.to_nat (64 / 8)) with 8%nat by (simpl; lia). 
+      rewrite Hget_mem. rewrite Hv0_bd at 1. rewrite Z.shiftr_0_r. reflexivity.
+    }
+  }
+  { (* 128 bit case *)
+    eapply Load128_R in H; try eassumption; try lia; [].
+    destruct H as (Hs' & Hls' & v & Heval_v & Hget_v & Hv_bd).
+    split; [exact Hs'|]. split; [solve_subsumed|].
+    exists v. split; [exact Heval_v|].
+    rewrite H3, E0.
+    exact Hget_v.
+  }
+  { (* 256 bit case *)
+    eapply Load256_R in H; try eassumption; try lia; [].
+    destruct H as (Hs' & Hls' & v & Heval_v & Hget_v & Hv_bd).
+    split; [exact Hs'|]. split; [solve_subsumed|].
+    exists v. split; [exact Heval_v|].
+    rewrite H3, E1.
+    exact Hget_v.
+  }
+Qed.
+
+(* looking up address a in state s returns value of idx i and state s' *)
+(* Then the new states correspond and eval i has value v in s' AND address a has value v in the machine state *)
+Lemma GetOperand_R {opts : symbolic_options_computed_opt} {descr:description} s m (HR: R s m) (so:OperationSize) (sa:AddressSize) (Hsa : sa = 64%N) a i s'
+  (H : GetOperand a s = Success (i, s'))
+  : R s' m /\ s :< s' /\ exists v, eval s' i v /\ DenoteOperand sa so m a = Some v.
+Proof using Type.
+  cbv [GetOperand DenoteOperand err] in *. break_innermost_match; inversion_ErrorT.
+  { eapply GetReg_R in H; intuition eauto. }
+  { eapply Load_R in H; intuition eauto. }    
+  {step_symex; repeat (eauto||econstructor). }
+Qed.
+
+Ltac step_GetOperand :=
+  match goal with
+  | H : GetOperand ?a ?s = Success (?i0, ?s') |- _ =>
+    let v := fresh "v" (*a*) in let Hv := fresh "H" v
+    in let Hi := fresh "H" i0 in let Heq := fresh H "eq" in
+    let Hs' := fresh "H" s' in let Hl := fresh "Hl" s' in
+    case (GetOperand_R s _ ltac:(eassumption) _ _ ltac:(reflexivity) _ _ _ H) as (Hs'&Hl&(v&Hi&Hv)); clear H
+  end.
+
+(* ----------------------------------------------*)
+(* SETTING OPERATIONS *)
+(* ----------------------------------------------*)
+
+Lemma interp_op_set_slice lo sz a b :
+  interp_op (set_slice lo sz) [a; b] = Some (bits_set_slice a b lo sz).
+Proof. reflexivity. Qed.
+
+
+Lemma SetMem_addr_mod m addr n v :                                                            
+  SetMem m (Z.land addr (Z.ones 64)) n v = SetMem m addr n v.
+Proof. 
+  cbv [SetMem Crypto.Util.Option.bind set_mem]. rewrite word_of_Z_land_ones_64. reflexivity. 
+Qed.
 
 Lemma store_R d s m (HR : R_mem d s m)
   (a : idx) va (Ha : eval d a va)
@@ -1015,85 +1194,22 @@ Proof using Type.
   setoid_rewrite (split_le_combine [b1; b2; b3; b4; b5; b6; b7]); trivial.
 Qed.
 
+Lemma subsumed_update_reg_with (s : symbolic_state) f
+  : s :< Symbolic.update_reg_with s f.
+Proof using Type. 
+  destruct s; cbv [Symbolic.update_reg_with]; cbn; exact (fun _ _ H => H). Qed.
 
-(* looking up address a in state s returns value of idx i and state s' *)
-(* Then the new states correspond and eval i has value v in s' AND address a has value v in the machine state *)
-Lemma GetOperand_R {opts : symbolic_options_computed_opt} {descr:description} s m (HR: R s m) (so:OperationSize) (sa:AddressSize) (Hsa : sa = 64%N) a i s'
-  (H : GetOperand a s = Success (i, s'))
-  : R s' m /\ s :< s' /\ exists v, eval s' i v /\ DenoteOperand sa so m a = Some v.
-Proof using Type.
-  cbv [GetOperand DenoteOperand err] in *. break_innermost_match; inversion_ErrorT.
-  { eapply GetReg_R in H; intuition eauto. }
-  {   
-    progress cbv [Load ret] in *.
-    repeat (cbv [err] in *; cbn [fst snd] in * || step_symex || Tactics.destruct_one_match_hyp || inversion_ErrorT || Prod.inversion_prod || subst).
-    (* 8/64 bit, scalar reg *)
-    { 
-        eapply Load64_R in HSv; try eassumption; [];
-        repeat (subst; destruct_head'_and; destruct_head'_ex).
-      repeat step_symex.
-      { repeat (eauto||econstructor). }
-      repeat (split; eauto; []).
-      rewrite Z.shiftr_0_r in Hi by lia.
-      case E as [E|E];
-        rewrite E in *; simpl Z.of_N in *.
-        (* case: one byte load *)
-        { cbv [get_mem Crypto.Util.Option.bind] in *.
-        destruct_one_match_hyp; Option.inversion_option.
-        epose proof length_load_bytes _ _ _ _ E0.
-        do 1 (destruct l; try solve [inversion H]).
-        eapply @nth_error_load_bytes with (i:=0%nat) in E0; [|clear;lia].
-        symmetry in E0; cbn [nth_error] in E0; simpl Z.of_nat in E0.
-        simpl load_bytes.
-        change (Pos.to_nat 1) with 1%nat.
-        cbv [load_bytes footprint List.map seq List.option_all].
-        setoid_rewrite E0.
-        eexists; split; eauto.
-        cbv [le_combine].
-        rewrite Z.shiftl_0_l, Z.lor_0_r.
-        change (Z.lor (Byte.byte.unsigned b) (Z.shiftl (le_combine l) 8) = x) in H4.
-        rewrite <-H4 in H5 at 2; rewrite H5; clear H4 H5.
-        f_equal.
-        rewrite <-Byte.byte.wrap_unsigned at 1; setoid_rewrite <-Z.land_ones; [|clear;lia].
-        rewrite <-Z.land_assoc.
-        change (Z.land (Z.ones 64) (Z.ones 8)) with (Z.ones 8).
-        rewrite Z.land_lor_distr_l.
-        bitblast.Z.bitblast. subst.
-        rewrite (Z.testbit_neg_r _ (_-8)) by lia; Btauto.btauto. }
-        (* case: 8 bytes load *)
-      { setoid_rewrite H4.
-        eexists; split; eauto; f_equal.
-        rewrite H5 at 1; trivial. }  
-    }
-    (* 128 bit, xmm *)
-    { eapply Load128_R in H; try eassumption; try lia; [];
-    repeat (subst; destruct_head'_and; destruct_head'_ex).
-    repeat (split; eauto; []). rewrite E0 in *. clear H5 H6. rewrite H8 in H4.
-    setoid_rewrite H7.
-    eexists; split; eauto; f_equal. exact H8. 
-      }
-    (* 256 bit, ymm *)
-    { eapply Load256_R in H; try eassumption; try lia; []; 
-    repeat (subst; destruct_head'_and; destruct_head'_ex).
-    repeat (split; eauto; []). rewrite E1 in *. clear H5 H6. rewrite H8 in H4.
-    setoid_rewrite H7.
-    eexists; split; eauto; f_equal. exact H8.  }
-  }
-  {step_symex; repeat (eauto||econstructor). }
-Qed.
+Lemma subsumed_update_flag_with (s : symbolic_state) f
+  : s :< Symbolic.update_flag_with s f.
+Proof using Type. 
+  destruct s; cbv [Symbolic.update_flag_with]; cbn; exact (fun _ _ H => H). Qed.
 
-
-Ltac step_GetOperand :=
-  match goal with
-  | H : GetOperand ?a ?s = Success (?i0, ?s') |- _ =>
-    let v := fresh "v" (*a*) in let Hv := fresh "H" v
-    in let Hi := fresh "H" i0 in let Heq := fresh H "eq" in
-    let Hs' := fresh "H" s' in let Hl := fresh "Hl" s' in
-    case (GetOperand_R s _ ltac:(eassumption) _ _ ltac:(reflexivity) _ _ _ H) as (Hs'&Hl&(v&Hi&Hv)); clear H
-  end.
+Lemma subsumed_update_mem_with (s : symbolic_state) f
+  : s :< Symbolic.update_mem_with s f.
+Proof using Type. 
+  destruct s; cbv [Symbolic.update_mem_with]; cbn; exact (fun _ _ H => H). Qed.
 
 Import Crypto.Util.ListUtil.
-
 Lemma combine_update_nth {A B} n (f : A -> A) (g : B -> B) xs ys :
   length xs = length ys ->
   combine (update_nth n f xs) (update_nth n g ys) = update_nth n (fun '(a, b) => (f a, g b)) (combine xs ys).
@@ -1107,193 +1223,220 @@ Lemma Forall2_update_nth_r {A B} (R : A -> B -> Prop) n f xs ys :
   Forall2 R xs ys ->                                                                                               
   (forall x y, nth_error xs n = Some x -> nth_error ys n = Some y -> R x y -> R x (f y)) ->                        
   Forall2 R xs (update_nth n f ys).         
-Proof.                                                                                                             
+Proof.
   intro H; revert n; induction H; intros [|n]; cbn.
-  - constructor.                                                                                                   
+  - constructor.
   - constructor; auto.
-  - constructor; [eapply H1; eauto; reflexivity | auto].                                                           
+  - constructor; [eapply H1; eauto; reflexivity | auto].
   - constructor; [auto | apply IHForall2; intros; eapply H1; eauto].
 Qed.
 
-(* 1. Full-width register write *)                                                                                 
-Lemma R_SetReg_full {opts : symbolic_options_computed_opt} {descr:description}
-   s m (HR : R s m) r i _tt s'
+Lemma reg_index_lt r : (N.to_nat (reg_index r) < length widest_registers)%nat.
+Proof. destruct r as [sr | vr]; [destruct sr | destruct vr]; vm_compute; lia. Qed.
+
+Lemma reg_size_offset_bounded (r : REG) :
+  (reg_size r + reg_offset r <= widest_reg_size_of r)%N.
+Proof. destruct r as [sr | vr]; [destruct sr | destruct vr]; vm_compute; intros; discriminate. Qed.
+
+Lemma R_regs_old_bound d sr mr (HR : R_regs d sr mr) r :
+  Tuple.nth_default 0 (N.to_nat (reg_index r)) mr =
+  Z.land (Tuple.nth_default 0 (N.to_nat (reg_index r)) mr)
+         (Z.ones (Z.of_N (widest_reg_size_of r))).
+Proof using Type.
+  unfold R_regs in HR.
+  rewrite Forall.Forall2_forall_iff_nth_error in HR.
+  specialize (HR (N.to_nat (reg_index r))).
+  rewrite nth_error_map, ListUtil.nth_error_combine in HR.
+  destruct (nth_error widest_registers (N.to_nat (reg_index r))) as [wr|] eqn:Hwr;
+    [| exfalso; apply nth_error_None in Hwr; pose proof (reg_index_lt r); lia ].
+  destruct (nth_error (Tuple.to_list _ sr) (N.to_nat (reg_index r))) as [[ix|]|] eqn:Hsr;
+  destruct (nth_error (Tuple.to_list _ mr) (N.to_nat (reg_index r))) as [conc|] eqn:Hmr;
+    cbn in HR; try contradiction.
+  - cbv [R_reg] in HR. destruct HR as [_ Hb].
+    rewrite <- Tuple.nth_default_to_list.
+    cbv [nth_default]. rewrite Hmr.
+    (* Goal: conc = conc & ones widest. Use Hb and widest_reg_size_of r = reg_size wr. *)
+    assert (widest_reg_size_of r = reg_size wr) as Hw.
+    { unfold widest_reg_size_of, widest_register_of_index, widest_register_of_index_opt.
+      replace (List.map ( @snd _ _) wide_reg_index_pairs) with widest_registers by reflexivity.
+      rewrite Hwr. reflexivity. }
+    rewrite Hw. exact Hb.
+  - cbv [R_reg] in HR. destruct HR as [_ Hb].
+    rewrite <- Tuple.nth_default_to_list. cbv [nth_default]. rewrite Hmr.
+    assert (widest_reg_size_of r = reg_size wr) as Hw.
+    { unfold widest_reg_size_of, widest_register_of_index, widest_register_of_index_opt.
+      replace (List.map ( @snd _ _) wide_reg_index_pairs) with widest_registers by reflexivity.
+      rewrite Hwr. reflexivity. }
+    rewrite Hw. exact Hb.
+Qed.
+ 
+(* works because Symbolic.set_reg just overwrites the reg slot. so the fun _ => v can replace bits_set_slice logic *)
+Lemma R_regs_set_reg d sr mr (HR : R_regs d sr mr) r (i : idx) v
+  (Hv : eval d i v)
+  (Hbound : v = Z.land v (Z.ones (Z.of_N (widest_reg_size_of r))))
+  : R_regs d (Symbolic.set_reg sr (reg_index r) i)
+  (Tuple.from_list_default 0%Z _
+  (ListUtil.update_nth (N.to_nat (reg_index r))
+  (fun _ => v)
+  (Tuple.to_list _ mr))).
+Proof. 
+  unfold R_regs, Symbolic.set_reg.
+  (* both sides become to_list ∘ update_nth — strip the tuple/list-default wrappers *)
+  unshelve erewrite 2 Tuple.from_list_default_eq, 2 Tuple.to_list_from_list;
+    try solve [rewrite ?ListUtil.length_set_nth, ?ListUtil.length_update_nth,
+                       ?Tuple.length_to_list; trivial].
+  unfold ListUtil.set_nth.
+  rewrite combine_update_nth by (rewrite !Tuple.length_to_list; reflexivity).
+  eapply Forall2_update_nth_r; [exact HR|].
+  intros x_old [sym_old conc_old] Hw _ HR_old.
+  (* extract width witness from the widths-list lookup *)
+  rewrite nth_error_map in Hw.
+  destruct (nth_error widest_registers (N.to_nat (reg_index r))) as [wr|] eqn:Hwr;
+    [cbn in Hw; inversion Hw; subst x_old | discriminate Hw].
+  (* widest_reg_size_of r = reg_size wr — same trick as in R_SetReg_full *)
+  assert (Hwidth : widest_reg_size_of r = reg_size wr).
+  { unfold widest_reg_size_of, widest_register_of_index, widest_register_of_index_opt.
+    replace (List.map ( @snd _ _) wide_reg_index_pairs) with widest_registers by reflexivity.
+    rewrite Hwr; reflexivity. }
+  rewrite <- Hwidth.
+  (* R_reg: split eval part from bitwidth part *)
+  split.
+  - intros i0 Hi0; inversion Hi0; subst; exact Hv.
+  - exact Hbound.
+Qed.
+
+(* bits_set_slice commutes with Z.land Z.ones *)
+Lemma bits_set_slice_bound (base v : Z) (shift sz W : N) :
+  (sz + shift <= W)%N ->
+  base = Z.land base (Z.ones (Z.of_N W)) ->
+  bits_set_slice base v shift sz =
+  Z.land (bits_set_slice base v shift sz) (Z.ones (Z.of_N W)).
+Proof using Type.
+  intros Hle Hbase. cbv [bits_set_slice].
+  rewrite Hbase at 2.
+  bitblast.Z.bitblast. 
+  rewrite Hbase. rewrite Z.land_spec, Z.testbit_ones_nonneg, (proj2 (Z.ltb_ge _ _)) by lia.
+  Btauto.btauto.
+Qed.
+
+(* bits_set_slice just clips v when v is widest with no offset *)
+Lemma bits_set_slice_widest (base v : Z) (shift sz W : N) :
+    shift = 0%N ->
+    sz = W ->
+    base = Z.land base (Z.ones (Z.of_N W)) ->
+    bits_set_slice base v shift sz = Z.land v (Z.ones (Z.of_N W)).
+Proof. 
+  intros. cbv [bits_set_slice]. subst. repeat rewrite Z.shiftl_0_r. 
+  rewrite H1. bitblast.Z.bitblast.
+Qed.
+
+(* used by R_SetRegSlice *)
+Lemma R_set_reg_via_splice {opts : symbolic_options_computed_opt} {descr : description}
+  s m (HR : R s m) r (i : idx) v
+  (Hi : eval s i (bits_set_slice (Tuple.nth_default 0 (N.to_nat (reg_index r)) (m : reg_state)) v
+                                  (reg_offset r) (reg_size r)))
+  : R (Symbolic.update_reg_with s (fun sr => Symbolic.set_reg sr (reg_index r) i))
+      (update_reg_with m (fun mr => set_reg mr r v)).
+Proof using Type.
+  destruct s as [d sr sf sm], m as [mr mf mm].
+  destruct HR as (Hok & Hregs & Hflags & Hmem).
+  cbv [R Symbolic.update_reg_with update_reg_with]; cbn in *.
+  ssplit; eauto.
+  unfold set_reg, index_and_shift_and_bitcount_of_reg.
+  erewrite ListUtil.update_nth_ext with
+    (g := fun _ => bits_set_slice (Tuple.nth_default 0 (N.to_nat (reg_index r)) mr) v
+                                   (reg_offset r) (reg_size r)).
+  2: { intros curv Hcurv.
+       f_equal.
+       rewrite <- Tuple.nth_default_to_list.
+       cbv [nth_default]. rewrite Hcurv. reflexivity. }
+
+  eapply R_regs_set_reg; [exact Hregs | exact Hi |].
+
+  pose proof (reg_size_offset_bounded r) as Hbnd.
+  pose proof (R_regs_old_bound _ _ _ Hregs r) as Hold_bnd.
+  apply bits_set_slice_bound; [exact Hbnd | exact Hold_bnd]. 
+Qed.
+  
+Lemma R_set_reg_overwrite {opts : symbolic_options_computed_opt} {descr : description}
+    s m (HR : R s m) r (i : idx) v
+    (Hoffset : reg_offset r = 0%N)
+    (Hwidest : reg_size r = widest_reg_size_of r)
+    (Hi : eval s i (Z.land v (Z.ones (Z.of_N (reg_size r)))))
+    : R (Symbolic.update_reg_with s (fun sr => Symbolic.set_reg sr (reg_index r) i))
+        (update_reg_with m (fun mr => set_reg mr r v)).
+Proof.
+  apply R_set_reg_via_splice with (v := v); [exact HR |].
+  rewrite Hoffset, Hwidest.
+  erewrite bits_set_slice_widest; eauto.
+  destruct s as [d sr sf sm]. 
+  destruct m as [mr mf mm]. 
+  rewrite (R_regs_old_bound d sr mr). rewrite Hwidest. bitblast.Z.bitblast.
+  unfold R in HR. destruct HR as (_ & HR & _). assumption. 
+Qed.
+
+(* Overwrite case: r is the widest register in its hierarchy. *)
+Lemma R_SetRegOverwrite {opts : symbolic_options_computed_opt} {descr:description}
+  s m (HR : R s m) r i _tt s'
   (Hoffset : reg_offset r = 0%N)
   (Hwidest : reg_size r = widest_reg_size_of r)
-  (H : Symbolic.SetReg r i s = Success (_tt, s'))
+  (H : Symbolic.SetRegOverwrite r i s = Success (_tt, s'))
   v (Hv : eval s i v)
   : exists m', Some (update_reg_with m (fun rs => set_reg rs r v)) = Some m'
     /\ R s' m' /\ s :< s'.
 Proof using Type.
-  eexists. repeat split;                                                                                                             
-    unfold SetReg in H; unfold set_reg, index_and_shift_and_bitcount_of_reg in *;                                    
-    rewrite Hoffset, Hwidest, N.eqb_refl, N.eqb_refl in *; simpl in H;  
-    step_symex;                               
-    cbn [fst snd] in H; cbv [SetRegFull] in H;                                                                       
-    inversion_ErrorT; Prod.inversion_prod; subst.
+  cbv [SetRegOverwrite index_and_shift_and_bitcount_of_reg] in H.
+  step_symex. rename v0 into i0. step_App; repeat (econstructor; eauto); cbv [fst snd] in *;
+  rewrite Z.shiftr_0_r in Hi0;
+  cbv [SetRegFull] in H; inversion_ErrorT; Prod.inversion_prod.
+  { subst. apply R_set_reg_overwrite; eauto. }
+  { eapply (subsumed_trans s s0 s'). 
+    -exact Hls0.
+    -rewrite <- H1; apply subsumed_update_reg_with. }
+Qed.
+
+(* Slice case: r is narrower than the widest register in its hierarchy.
+   No precondition on offset/size: SetRegSlice always works correctly. *)
+Lemma R_SetRegSlice {opts : symbolic_options_computed_opt} {descr:description}
+  s m (HR : R s m) r i _tt s'
+  (H : Symbolic.SetRegSlice r i s = Success (_tt, s'))
+  v (Hv : eval s i v)
+  : exists m', Some (update_reg_with m (fun rs => set_reg rs r v)) = Some m'
+    /\ R s' m' /\ s :< s'.
+Proof using Type.
+  cbv [SetRegSlice index_and_shift_and_bitcount_of_reg] in H.
+  repeat step_symex; cbv [fst snd] in *; rename v0 into i0;
+  step_GetRegFull; 
+  eapply App_R with (m := m) (v := bits_set_slice v0 v (reg_offset r) (reg_size r)) in HSv0; repeat (econstructor; eauto);
+  cbv [SetRegFull] in H; inversion_ErrorT; Prod.inversion_prod; eauto.
   {
-    rewrite !Z.shiftl_0_r.
-    step_App. { repeat eauto || econstructor. }
-    rewrite !Z.shiftr_0_r in Hv0.
-
-    destruct s0 as [d0 sr0 sf0 sm0]; destruct Hs0 as (Hok0 & Hregs0 & Hflags0 & Hmem0).
-    cbv [R update_reg_with Symbolic.update_reg_with]; cbn.
-    split; [| split; [ |split]]; eauto.
-    unfold R_regs, Symbolic.set_reg.
-
-    unshelve erewrite 2Tuple.from_list_default_eq, 2Tuple.to_list_from_list;
-    try solve [rewrite ?Crypto.Util.ListUtil.length_set_nth,
-              ?Crypto.Util.ListUtil.length_update_nth,                                                              
-              ?Tuple.length_to_list; trivial].
-
-    unfold ListUtil.set_nth. rewrite combine_update_nth.
-    2: repeat rewrite Tuple.length_to_list; reflexivity.
-    eapply Forall2_update_nth_r.
-    { exact Hregs0. }
-    intros x_old v_old Hw Hy HR_old. 
-    destruct v_old as [sym_old conc_old].
-
-    cbv [R_reg] in *. destruct HR_old as [_ Hbits_old].                                                                
-    (* extract width from Hw *)                                                                                        
-    rewrite nth_error_map in Hw.                                                                                       
-    destruct (nth_error widest_registers (N.to_nat (reg_index r))) as [wr|] eqn:Hwr;                                   
-      [cbn in Hw; inversion Hw; subst x_old | discriminate Hw].                                                        
-    (* show widest_reg_size_of r = reg_size wr *)                                                                      
-    assert (Hwidth : widest_reg_size_of r = reg_size wr).                                                              
-    { unfold widest_reg_size_of, widest_register_of_index, widest_register_of_index_opt.                               
-      replace (List.map ( @snd _ _) wide_reg_index_pairs) with widest_registers by reflexivity.  (* both are Eval lazy, should reduce *)                                                       
-      rewrite Hwr. reflexivity. }               
-    (* Z.ldiff conc_old ... = 0 because conc_old fits in width bits *)                                                 
-    assert (Hldiff : Z.ldiff conc_old (Z.ones (Z.of_N (widest_reg_size_of r))) = 0).
-    { rewrite Hwidth, Hbits_old. bitblast.Z.bitblast. }                                                                         
-    rewrite Hldiff, Z.lor_0_r.              
-    split.                                                                                                             
-    - intros i0 Hi0; inversion Hi0; subst. exact Hv0.                                                                  
-    - bitblast.Z.bitblast.
+    subst. destruct HSv0 as (HR1 & Hsubs1 & Heval1).
+    apply R_set_reg_via_splice; eauto.
   }
   {
-    step_App. { repeat eauto || econstructor. }
-    subst. simpl. exact Hls0.
+    destruct HSv0 as (HR1 & Hsubs1 & Heval1).
+    eapply (subsumed_trans s s1 s'). 
+    -exact Hsubs1.
+    -rewrite <- H1; apply subsumed_update_reg_with.
   }
 Qed.
 
-Lemma reg_size_offset_bounded (r : REG) :                                                                          
-  (reg_size r + reg_offset r <= widest_reg_size_of r)%N.
-Proof. destruct r as [sr | vr]; [destruct sr | destruct vr]; vm_compute; intros; discriminate. Qed.   
-  
-(* 2. Partial register write *)                     
-Lemma R_SetReg_partial {opts : symbolic_options_computed_opt} {descr:description}
-  s m (HR : R s m) r i _tt s'                                                  
-  (Hpartial : ((reg_offset r =? 0)%N && (reg_size r =? widest_reg_size_of r)%N)%bool = false)                      
-  (H : Symbolic.SetReg r i s = Success (_tt, s'))                                                                  
-  v (Hv : eval s i v)                   
-  : exists m', Some (update_reg_with m (fun rs => set_reg rs r v)) = Some m'                                       
-  /\ R s' m' /\ s :< s'.
-Proof using Type.                                                                                                  
-  eexists. repeat split.                                                                                           
-  { (* R s' m' *)                                                                                                  
-    unfold SetReg in H. unfold set_reg, index_and_shift_and_bitcount_of_reg in *.                                  
-    rewrite Hpartial in H.                                                                                         
-    (* H is now: (old <- GetRegFull rn; v_new <- App (set_slice lo sz, [old; i]); SetRegFull rn v_new) s *)        
-                                            
-    (* Process GetRegFull: reads old register, state unchanged *)                                                  
-    repeat step_symex.
-    cbn [fst snd] in HSv0.
-    
-    cbv [GetRegFull some_or] in HSold.                                                                                 
-    pose proof (get_reg_R s _ HR (reg_index r)) as Hr_old.                                                             
-    destruct (Symbolic.get_reg (symbolic_reg_state s) (reg_index r)) eqn:Hgreg;                                        
-      [| discriminate HSold].               
-    inversion HSold; subst s0. clear HSold.
-    specialize (Hr_old _ eq_refl). destruct Hr_old as (old_val & Heval_old & Hold_eq).                                 
-                                            
-    (* App_R on set_slice *)                                                                                           
-    eapply App_R in HSv0 as (HRs1 & Hsub1 & Heval_v0).
-    2: { exact HR. }
-    2: { subst old. repeat (eauto || econstructor). }                                                               
-                                                                                                                        
-    (* SetRegFull *)                        
-    cbn [fst snd] in H. cbv [SetRegFull] in H.                                                                         
-    inversion_ErrorT; Prod.inversion_prod; subst.        
-    destruct s1 as [d1 sr1 sf1 sm1].                                                                                   
-    destruct HRs1 as (Hok1 & Hregs1 & Hflags1 & Hmem1).
-    cbv [R update_reg_with Symbolic.update_reg_with]; cbn.                                                             
-    split; [| split; [| split]]; eauto.         
-                                                                                                                      
-    (* R_regs *)    
-    unfold R_regs, Symbolic.set_reg.                                                                                   
-    unshelve erewrite 2Tuple.from_list_default_eq, 2Tuple.to_list_from_list;
-      try solve [rewrite ?Crypto.Util.ListUtil.length_set_nth,                                                         
-                ?Crypto.Util.ListUtil.length_update_nth,
-                ?Tuple.length_to_list; trivial].
-    unfold ListUtil.set_nth. rewrite combine_update_nth.                                                               
-    2: repeat rewrite Tuple.length_to_list; reflexivity.
-    eapply Forall2_update_nth_r.                                                                                       
-    { exact Hregs1. }                           
-    intros x_old v_old Hw Hy HR_old.                                                                                   
-    destruct v_old as [sym_old conc_old].
-    cbv [R_reg] in *. destruct HR_old as [_ Hbits_old].                                                                
-    rewrite nth_error_map in Hw.                
-    destruct (nth_error widest_registers (N.to_nat (reg_index r))) as [wr|] eqn:Hwr;                                   
-      [cbn in Hw; inversion Hw; subst x_old | discriminate Hw].
-    assert (Hwidth : widest_reg_size_of r = reg_size wr).                                                              
-    { unfold widest_reg_size_of, widest_register_of_index, widest_register_of_index_opt.
-      replace (List.map ( @snd _ _) wide_reg_index_pairs) with widest_registers                                         
-        by reflexivity.                                                                                                
-      rewrite Hwr. reflexivity. }
-    split.                                                                                                             
-    - intros i0 Hi0; inversion Hi0; subst. simpl in Heval_v0.
-      replace conc_old with (Tuple.nth_default 0 (N.to_nat (reg_index r)) (machine_reg_state m)).
-      2: { rewrite nth_error_combine in Hy.
-        destruct (nth_error (Tuple.to_list 100 sr1) (N.to_nat (reg_index r))) eqn:Hsr;
-          [| discriminate Hy].
-        destruct (nth_error (Tuple.to_list 100 (machine_reg_state m)) (N.to_nat (reg_index r))) eqn:Hm;
-          [| discriminate Hy].                  
-        inversion Hy; subst conc_old.               
-        rewrite <- Tuple.nth_default_to_list. unfold nth_default. rewrite Hm. reflexivity.  
-      } 
-      cbv [Tuple.nth_default] in Heval_v0. exact Heval_v0.
-    -
-      pose proof (reg_size_offset_bounded r).     
-      rewrite Hwidth in *.                    
-      rewrite Hbits_old.
-      bitblast.Z.bitblast.     
-  }
-  {
-    unfold SetReg, index_and_shift_and_bitcount_of_reg in H.
-    rewrite Hpartial in H.                      
-    repeat step_symex.
-    cbv [fst snd] in HSv0.
-    cbv [fst snd SetRegFull] in H.
-    pose proof (get_reg_R s _ HR (reg_index r)) as Hr_old.
-    cbv [GetRegFull some_or] in HSold.
-    eapply App_R in HSv0.
-    {
-      inversion_ErrorT; Prod.inversion_prod; subst.
-      destruct HSv0 as [_ [Hsub _]].
-      destruct (Symbolic.get_reg (symbolic_reg_state s) (reg_index r));                                                  
-      [| discriminate HSold].                                                                                          
-      inversion HSold; subst s0.
-      unfold Symbolic.update_reg_with; simpl.                                                                            
-      exact Hsub. 
-    }
-    {
-      destruct (Symbolic.get_reg (symbolic_reg_state s) (reg_index r)). 
-      inversion HSold. rewrite <- H2. exact HR.
-      discriminate HSold.
-    }
-    {
-      destruct (Symbolic.get_reg (symbolic_reg_state s) (reg_index r)) eqn:Hgreg;
-        [| discriminate HSold].                                                                                          
-      (* pose proof (get_reg_R s _ HR (reg_index r)) as Hr_old. *)
-      inversion HSold. subst s0. 
-      specialize (Hr_old _ eq_refl). destruct Hr_old as (old_val & Heval_old & Hold_eq).  
-      subst old.                                                                                       
-      eapply ENod with (args' := [old_val; v]).                                                                          
-      - constructor; [exact Heval_old | constructor; [exact Hv | constructor]].                                          
-      - cbn [interp_op]. f_equal. rewrite <- Hold_eq. reflexivity.
-    }           
-  }
+Lemma R_SetReg {opts : symbolic_options_computed_opt} {descr:description}
+  s m (HR : R s  m) r i _tt s'
+  (H : Symbolic.SetReg r i s = Success (_tt, s'))
+  v (Hv : eval s i v)
+  : exists m', Some (update_reg_with m (fun rs => set_reg rs r v)) = Some m'
+    /\ R s' m' /\ s :< s'.
+Proof. 
+  destruct ((reg_offset r =? 0)%N && (reg_size r =? widest_reg_size_of r)%N)%bool eqn:Hb.
+  - apply andb_prop in Hb. destruct Hb as [Hoffset Hwidest]. 
+  unfold SetReg, index_and_shift_and_bitcount_of_reg in H. 
+  rewrite Hoffset, Hwidest in H. simpl in H.
+  apply Neqb_ok in Hoffset, Hwidest.
+  eapply R_SetRegOverwrite in H; eauto. 
+  - unfold SetReg, index_and_shift_and_bitcount_of_reg in H. 
+    rewrite Hb in H.
+    eapply R_SetRegSlice in H; eauto.
 Qed.
 
 Lemma DenoteAddressLandOnes sa m a addr :
@@ -1305,150 +1448,327 @@ Proof.
   intros. subst. unfold DenoteAddress. apply H.
 Qed.
 
-Lemma le_split_app n1 n2 v :                   
-  le_split (n1 + n2) v = le_split n1 v ++ le_split n2 (Z.shiftr v (8 * Z.of_nat n1)).                              
-Proof.                                                                                                             
-  rewrite <- (firstn_skipn n1 (le_split (n1 + n2) v)).                                                             
-rewrite skipn_le_split'. Admitted.
-  (* rewrite List.firstn_le_split.                                                                                    
-  rewrite Nat.min_l by lia. reflexivity. *)
-(* Qed. *)
-
-
-Lemma store_bytes_app (m: mem_state) a bs1 bs2 m1 m2 :                                     
-  store_bytes m a bs1 = Some m1 ->                                                                                 
-  store_bytes m1 (word.add a (word.of_Z (Z.of_nat (length bs1)))) bs2 = Some m2 ->                                
-  store_bytes m a (bs1 ++ bs2) = Some m2. 
-Proof. Admitted.
-
-
-(* n1 n2 are in bytes *)
-(* setting lower n1 bytes to lower part of v gives state m1 *)
-(* setting upper n2 bytes to upper shifted part of v gives state m2 *)
-(* then setting all bytes to v simultaneously gives m2. *)
-Lemma SetMem_compose m addr n1 n2 v m1 m2 :                                       
-  SetMem m addr n1 (Z.land v (Z.ones (8 * Z.of_nat n1))) = Some m1 ->                                              
-  SetMem m1 (addr + Z.of_nat n1) n2 (Z.shiftr v (8 * Z.of_nat n1)) = Some m2 ->                                    
-  SetMem m addr (n1 + n2) v = Some m2.                                                                             
-Proof.
-  cbv [SetMem set_mem Crypto.Util.Option.bind].                                                                    
-  intros H1 H2.                                                                                                    
-  destruct (store_bytes _ _ (le_split n1 _)) eqn:Hs1 in H1; [| discriminate].                                      
-  inversion H1; subst m1; clear H1.                                                                                
-  destruct (store_bytes _ _ (le_split n2 _)) eqn:Hs2 in H2; [| discriminate].                                      
-  inversion H2; subst m2; clear H2.                                                                                
-  (* Need: store_bytes m (word.of_Z addr) (le_split (n1+n2) v) = Some m0 *)
-  rewrite le_split_app. rewrite Z.land_ones in Hs1 by lia. 
-  erewrite store_bytes_app.
-  2 : { rewrite le_split_mod. replace (Z.of_nat n1 * 8) with (8 * Z.of_nat n1) by lia. exact Hs1. }
-  2 : { rewrite length_le_split. rewrite <- word.ring_morph_add. exact Hs2. }
-  reflexivity.
+Lemma byte_wrap_bounds w n
+	(H : Z.of_nat n > 0) :
+	Byte.byte.wrap (w mod 2^ (8 * Z.of_nat n)) = Byte.byte.wrap w.
+Proof. 
+	unfold Byte.byte.wrap. eapply Z.mod_mod_divide.
+	 rewrite Z.pow_mul_r; [apply Zpow_facts.Zpower_divide; lia | lia | lia]. 
 Qed.
-  
-  (* 3. Memory write *)                                                                                              
-Lemma R_SetMem {opts : symbolic_options_computed_opt} {descr:description} s m (HR : R s m) (sz : OperationSize) (sa : AddressSize)                             
-  a i _tt s'
-  (Hsa : sa = 64%N)                      
-  (H : Symbolic.Store a i s = Success (_tt, s'))                                                                   
+
+Lemma byte_of_Z_bounds w n (H : Z.of_nat n > 0) :
+      Byte.byte.of_Z (Z.land w (Z.ones (8 * Z.of_nat n))) = Byte.byte.of_Z w.
+  Proof.
+		assert (forall a b, Byte.byte.wrap a = Byte.byte.wrap b -> Byte.byte.of_Z a = Byte.byte.of_Z b) as byte_wrap.
+		{
+		intros a b H2. unfold Byte.byte.of_Z.
+    generalize (Byte.byte.Byte_of_N_of_mod_not_None a).
+    generalize (Byte.byte.Byte_of_N_of_mod_not_None b).
+    rewrite H2.
+    intros f1 f2.
+    destruct (Byte.of_N (Z.to_N (Byte.byte.wrap b))).
+    - reflexivity.
+    - exfalso. exact (f1 eq_refl).
+		}
+    rewrite Z.land_ones by lia.
+    apply byte_wrap.
+    apply byte_wrap_bounds. lia.
+  Qed.
+
+Lemma le_split_bounds n v :
+			le_split n (Z.land v (Z.ones (8 * Z.of_nat n))) = le_split n v.
+Proof.
+	revert v; induction n; intros v.
+	{ reflexivity. }
+	{ change (le_split (S n) ?x) with (Byte.byte.of_Z x :: le_split n (Z.shiftr x 8)).
+		rewrite byte_of_Z_bounds. 
+	f_equal. rewrite Z.shiftr_land by lia.
+  replace (Z.shiftr (Z.ones (8 * Z.of_nat (S n))) 8) with (Z.ones (8 * Z.of_nat n)).
+	{ apply IHn. }
+	{ bitblast.Z.bitblast. }
+	{ lia. }
+	}
+Qed.
+
+Lemma SetMem_bounds m addr nbytes v : 
+			SetMem m addr nbytes (Z.land v (Z.ones (8 * Z.of_nat nbytes))) = SetMem m addr nbytes v.
+Proof. 
+			 intros. unfold SetMem, Crypto.Util.Option.bind in *. destruct (set_mem m addr nbytes v) eqn:H;
+			 unfold set_mem in *; rewrite le_split_bounds; rewrite H; reflexivity. 
+Qed.
+
+Lemma le_split_app n1 n2 v :
+  le_split (n1 + n2) v = le_split n1 v ++ le_split n2 (Z.shiftr v (8 * Z.of_nat n1)).
+Proof. 
+			 revert n2 n1 v. induction n1.
+			 { intros. simpl. rewrite Z.shiftr_0_r. reflexivity. }
+			 { intros. 
+			 change (le_split (S n1 + n2) ?x) with (Byte.byte.of_Z x :: le_split (n1 + n2) (Z.shiftr x 8)).
+			 change (le_split (S n1) ?x) with (Byte.byte.of_Z x :: le_split n1 (Z.shiftr x 8)).
+			 rewrite IHn1. 
+			 replace (Z.shiftr (Z.shiftr v 8) (8 * Z.of_nat n1)) with (Z.shiftr v (8 * Z.of_nat (S n1))). reflexivity.
+			 bitblast.Z.bitblast. }
+Qed.
+
+Lemma load_bytes_unchecked_store_bytes_covered (m : mem_state) (a : word64) bs (a2 : word64) n2 r1 r2 :
+  load_bytes m a (length bs) = Some r1 ->
+  load_bytes (unchecked_store_bytes m a bs) a2 n2 = Some r2 ->
+  exists r, load_bytes m a2 n2 = Some r.
+Proof.
+  intros H1 H2.
+  apply Memory.load_bytes_all.
+  intros i Hi.
+  (* From H2: address (a2 + i) is accessible in m1 *)
+  pose proof (Memory.nth_error_load_bytes _ _ _ _ H2 i Hi) as Hm1.
+  (* nth_error r2 i is Some something *)
+  destruct (List.nth_error r2 i) as [b|] eqn:Er2.
+  2: { apply List.nth_error_None in Er2.
+       erewrite Memory.length_load_bytes in Er2 by exact H2. lia. }
+  symmetry in Hm1.
+  (* Hm1 : map.get m1 (a2+i) = Some b *)
+  cbv [unchecked_store_bytes] in Hm1.
+  rewrite Properties.map.get_putmany_dec in Hm1.
+  destruct (map.get (map.of_list_word_at a bs) (word.add a2 (word.of_Z (Z.of_nat i))))
+    as [b'|] eqn:Eov.
+  - (* In the overlay: addr is in footprint a (length bs); use H1 *)
+    rewrite OfListWord.map.get_of_list_word_at in Eov.
+    apply List.nth_error_Some_bound_index in Eov.
+    set (j := Z.to_nat (word.unsigned (word.sub (word.add a2 (word.of_Z (Z.of_nat i))) a))) in *.
+    pose proof (Memory.nth_error_load_bytes _ _ _ _ H1 j Eov) as Hm.
+    (* Hm : nth_error r1 j = map.get m (a + j) *)
+    (* Need: a + j = a2 + i  (in word arithmetic) *)
+    assert (Haddr : word.add a (word.of_Z (Z.of_nat j)) =
+                    word.add a2 (word.of_Z (Z.of_nat i))).
+    { subst j. rewrite Z2Nat.id by apply word.unsigned_range.
+      rewrite word.of_Z_unsigned. ring. }
+    rewrite Haddr in Hm.
+    destruct (List.nth_error r1 j) eqn:Er1.
+    + eauto.
+    + apply List.nth_error_None in Er1.
+      erewrite Memory.length_load_bytes in Er1 by exact H1. lia.
+  - (* Not in overlay: map.get m1 = map.get m *)
+    eauto.
+Qed.
+
+
+Lemma store_bytes_app (m: mem_state) a bs1 bs2 m1 m2 :
+    (Z.of_nat (length bs1) + Z.of_nat (length bs2) <= 2^64)%Z ->
+    store_bytes m a bs1 = Some m1 ->
+    store_bytes m1 (word.add a (word.of_Z (Z.of_nat (length bs1)))) bs2 = Some m2 ->
+    store_bytes m a (bs1 ++ bs2) = Some m2.
+  Proof.
+    intros Hlen H1 H2.
+    cbv [store_bytes] in *.
+    destruct (load_bytes m a (length bs1)) as [r1|] eqn:E1; [|discriminate].
+    set (m1' := unchecked_store_bytes m a bs1) in *.
+    assert (Hm1 : m1' = m1) by
+      exact (f_equal (fun x => match x with Some y => y | None => m end) H1).
+    subst m1.
+    destruct (load_bytes m1' _ (length bs2)) as [r2|] eqn:E2; [|discriminate].
+    set (m2' := unchecked_store_bytes m1' _ bs2) in *.
+    assert (Hm2 : m2' = m2) by
+      exact (f_equal (fun x => match x with Some y => y | None => m1' end) H2).
+    subst m2.
+    rewrite app_length.
+    (* Guard *)
+    edestruct (load_bytes_unchecked_store_bytes_covered m a bs1 _ _ _ _ E1 E2) as [r3 E3].
+    unfold load_bytes. rewrite footprint_app, List.map_app.
+    pose proof E1 as E1'. unfold load_bytes in E1'.
+    pose proof E3 as E3'. unfold load_bytes in E3'.
+    erewrite option_all_app by eassumption.
+    (* Compose *)
+    f_equal. subst m1' m2'.
+    cbv [unchecked_store_bytes].
+    rewrite OfListWord.map.of_list_word_at_app.
+    rewrite Properties.map.putmany_assoc.
+    rewrite Properties.map.disjoint_putmany_commutes. reflexivity.
+    eapply OfListWord.map.adjacent_arrays_disjoint. lia.
+  Qed.
+
+
+(* Writing lower n1 bytes, then upper n2 bytes, equals writing all (n1+n2) bytes. *)
+Lemma SetMem_compose m addr n1 n2 v m1 m2 :
+	(Z.of_nat n1 + Z.of_nat n2 <= 2^64)%Z ->
+  SetMem m addr n1 (Z.land v (Z.ones (8 * Z.of_nat n1))) = Some m1 ->
+  SetMem m1 (addr + Z.of_nat n1) n2 (Z.shiftr v (8 * Z.of_nat n1)) = Some m2 ->
+  SetMem m addr (n1 + n2) v = Some m2.
+Proof.
+  cbv [SetMem set_mem Crypto.Util.Option.bind].
+  intros H H1 H2.
+  destruct (store_bytes _ _ (le_split n1 _)) eqn:Hs1 in H1; [| discriminate].
+  inversion H1; subst m1; clear H1.
+  destruct (store_bytes _ _ (le_split n2 _)) eqn:Hs2 in H2; [| discriminate].
+  inversion H2; subst m2; clear H2.
+  rewrite le_split_app. rewrite le_split_bounds in Hs1.
+  erewrite store_bytes_app.
+  - reflexivity.
+	- rewrite !length_le_split. lia.
+  - exact Hs1.
+  - rewrite length_le_split. rewrite <- word.ring_morph_add. exact Hs2.
+Qed.
+
+Lemma R_Store_of_idx {opts : symbolic_options_computed_opt} {descr:description}
+  {sa : AddressSize} (Hsa : sa = 64%N)
+  n s m (HR : R s m)
+	(Hlen : Z.of_nat (8 * n) <= 2^64%Z)
+  (addr : idx) va (Ha : eval s addr va)
+  (i : idx) v (Hv : eval s i v)
+  _tt s' (H : Store_of_idx n addr i s = Success (_tt, s'))
+  : exists m', SetMem m va (8 * n)%nat v = Some m' /\ R s' m' /\ s :< s'.
+Proof using Type.
+  revert s m HR addr va Ha i v Hv _tt s' H.
+  induction n as [|n' IH]; intros.
+  { (* base: Store_of_idx 0 = ret tt *)
+    cbn [Store_of_idx] in H.
+    inversion_ErrorT; Prod.inversion_prod; subst.
+		unfold ret in H; inversion H; subst.
+    exists m. split; [ cbv; reflexivity | split; eauto].
+  }
+  { (* step: recursive Store_of_idx n' + App offset + App addr_k + App chunk + Store64 *)
+    cbn [Store_of_idx] in H.
+    repeat (cbn [fst snd] in * || step_symex || Tactics.destruct_one_match_hyp
+            || inversion_ErrorT || Prod.inversion_prod || subst).
+    (* IH: store the low n'*64 bits *)
+    assert (Hv_low : Z.land v (Z.ones (64 * Z.of_nat n')) =
+                     Z.land (Z.land v (Z.ones (64 * Z.of_nat n')))
+                            (Z.ones (64 * Z.of_nat n'))).
+    { bitblast.Z.bitblast. }
+
+    eapply IH in HSx as (m1 & Hset1 & HR1 & Hsub1);
+      try eassumption; try exact Hv_low.
+			2: { assert  (Z.of_nat (8 * n') <= Z.of_nat (8 * S n')) as Q; lia. }
+    (* App_R for offset const (8 * n') *)
+    eapply App_R in HSoffset as (HR2 & Hsub2 & Heval_offset); [| exact HR1 | repeat (econstructor; eauto)].
+    (* App_R for addr_k = addr + offset *)
+    eapply App_R in HSaddr_k as (HR3 & Hsub3 & Heval_addr_k); [|exact HR2 |  repeat (econstructor; eauto)].
+    cbn [fold_right] in Heval_addr_k. rewrite Z.add_0_r in Heval_addr_k.
+
+    (* App_R for chunk = slice (64*n') 64 [i] *)
+    assert (Hchunk_val : Z.land (Z.shiftr v (Z.of_N (64 * N.of_nat n'))) (Z.ones (Z.of_N 64))
+                       = Z.land (Z.shiftr v (64 * Z.of_nat n')) (Z.ones 64)).
+    { replace (Z.of_N (64 * N.of_nat n')) with (64 * Z.of_nat n') by lia.
+      replace (Z.of_N 64) with 64 by lia. reflexivity. }
+    eapply App_R in HSchunk as (HR4 & Hsub4 & Heval_chunk); [|exact HR3 |  repeat (econstructor; eauto)].
+
+    (* Store64_R for the chunk at addr + 8*n' *)
+    set (chunk_val := Z.land (Z.shiftr v (64 * Z.of_nat n')) (Z.ones 64)).
+    assert (Hchunk_bounded : chunk_val = Z.land chunk_val (Z.ones 64)). { unfold chunk_val. bitblast.Z.bitblast. }
+    eapply Store64_R with
+      (v' := Z.shiftr v (8 * Z.of_nat (8 * n')))
+      (va := Z.land (va + 8 * Z.of_nat n') (Z.ones 64))
+      in H; try eassumption; try bitblast.Z.bitblast.
+		2: { apply Hsub4. replace (Z.ones (Z.of_N 64)) with (Z.ones 64) by eauto. exact Heval_addr_k. }
+
+    destruct H as (m2 & Hset2 & HR5 & Hsub5).
+    (* Compose the two SetMem operations *)
+    rewrite SetMem_addr_mod in Hset2.
+    exists m2. split; [|split; [exact HR5|]].
+    { (* SetMem m va (8 * S n') v = Some m2 *)
+		
+      replace (8 * S n')%nat with (8 * n' + 8)%nat by lia.
+      eapply SetMem_compose.
+			{ replace (Z.of_nat (8 * n') + Z.of_nat 8) with ( Z.of_nat (8 * S n')) by lia.
+				 exact Hlen. }
+      { rewrite SetMem_bounds. exact Hset1. }
+      { replace (Z.of_nat (8 * n')) with (8 * Z.of_nat n') by lia.
+        replace (8 * (8 * Z.of_nat n')) with (8 * Z.of_nat (8 * n')) by lia.
+        exact Hset2. }
+    }
+    { solve_subsumed. } 
+  }
+Qed.
+
+(* 128-bit store corollary *)
+Corollary R_Store128_of_idx {opts : symbolic_options_computed_opt} {descr:description}
+  {sa : AddressSize} (Hsa : sa = 64%N)
+  s m (HR : R s m) (addr : idx) va (Ha : eval s addr va)
+  (i : idx) v (Hv : eval s i v)
+  _tt s' (H : Store128_of_idx addr i s = Success (_tt, s'))
+  : exists m', SetMem m va 16%nat v = Some m' /\ R s' m' /\ s :< s'.
+Proof using Type.
+  cbv [Store128_of_idx] in H. eapply R_Store_of_idx with (n := 2%nat); eauto. lia.
+Qed.
+
+(* 256-bit store corollary *)
+Corollary R_Store256_of_idx {opts : symbolic_options_computed_opt} {descr:description}
+  {sa : AddressSize} (Hsa : sa = 64%N)
+  s m (HR : R s m) (addr : idx) va (Ha : eval s addr va)
+  (i : idx) v (Hv : eval s i v)
+  _tt s' (H : Store256_of_idx addr i s = Success (_tt, s'))
+  : exists m', SetMem m va 32%nat v = Some m' /\ R s' m' /\ s :< s'.
+Proof using Type.
+  cbv [Store256_of_idx] in H. eapply R_Store_of_idx with (n := 4%nat); eauto. lia.
+Qed.
+
+
+Lemma R_Store {opts : symbolic_options_computed_opt} {descr:description}
+  {sz : OperationSize} {sa : AddressSize} (Hsa : sa = 64%N)
+  s m (HR : R s m) a i _tt s'
+  (H : Symbolic.Store a i s = Success (_tt, s'))
   v (Hv : eval s i v)
-  : exists m', SetMem m (DenoteAddress sa m a) (N.to_nat (operand_size a sz / 8)) v = Some m'                      
-  /\ R s' m' /\ s :< s'.  
-Proof using Type.                                                                                                  
-    progress cbv [Store] in *.
-    rewrite Hsa in *. clear sa Hsa.                                                                                 
-    (* case split on operand_size *)
-    destruct_one_match_hyp; cbv [err] in *; [| destruct_one_match_hyp; [| destruct_one_match_hyp]];                  
-      try inversion_ErrorT.
-    { (* 8/64 bit store *)
-      repeat (step_symex; cbn [fst snd] in *).
-      eapply Load64_R in HSold; eauto;                                                                       
-      repeat (subst; destruct_head'_ex; destruct_head'_and).                                                       
-      repeat (step_symex; cbn [fst snd] in *).                                                                       
-      { repeat (eauto || econstructor). }
-      { repeat (eauto || econstructor). }                                                                            
-      rewrite !Z.shiftl_0_r, ?Z.shiftr_0_r, <-Z.land_assoc, Z.land_diag in *.
-      case E as [E|E]; rewrite E in *; simpl Z.of_N in *.                                                            
-      + (* 8-bit *)                                                                                                  
-      eapply Store64_R with (v':=Z.lor (Z.land v (Z.ones 8)) (Z.ldiff x (Z.ones 8))) in H;
-      try eassumption; eauto with nocore; try solve [rewrite H5; bitblast.Z.bitblast].                           
-      destruct_head'_ex; destruct_head'_and.
-      cbv [SetMem Crypto.Util.Option.bind update_mem_with] in *;                                                   
-      destruct set_mem eqn:? in *; Option.inversion_option; subst.                                               
-      erewrite store8; eauto 9.                                                                                    
-      + (* 64-bit *)                                                                                                 
-      eapply Store64_R with (v':=v) in H;                                                                          
-      try eassumption; eauto with nocore; try solve [rewrite H5; bitblast.Z.bitblast].
-      destruct_head'_ex; destruct_head'_and. setoid_rewrite H. eauto 9.                                            
+  : exists m', SetMem m (DenoteAddress sa m a) (N.to_nat (operand_size a sz / 8)) v = Some m'
+              /\ R s' m' /\ s :< s'.
+Proof. 
+  cbv [Store] in H.
+  step_symex; cbv [fst snd] in *.
+  step_Address. rename x into va.
+  repeat (destruct_one_match_hyp; try discriminate H).
+  repeat step_symex; cbv [fst snd] in *.
+  { (* 8 and 64 bit cases *)
+    eapply Load64_R in HSold; [|eassumption|eassumption].
+    destruct HSold as (Hs1 & old_val & Heval_old & Hget_old & Hbound_old); subst.
+    step_App; [repeat (econstructor; eauto)|].
+    step_App; [repeat (econstructor; eauto)|].
+    rewrite !Z.shiftl_0_r, !Z.shiftr_0_r in *.
+    destruct E as [E|E]; rewrite E in *.
+    { (* 8-bit store: read-modify-write *)
+      eapply Store64_R with (v' := Z.lor (Z.land v (Z.ones 8)) (Z.ldiff old_val (Z.ones 8))) in H;
+        try eassumption; eauto with nocore;
+        try solve [rewrite Hbound_old; bitblast.Z.bitblast].
+      destruct H as (m' & Hset & HR' & Hsub').
+      cbv [SetMem Crypto.Util.Option.bind update_mem_with] in *.
+      destruct set_mem eqn:? in *; Option.inversion_option; subst.
+      erewrite store8; eauto 9.
     }
-    { Admitted. (* 128-bit store *)                                                                                            
-      (* Step through: App(slice 0 64), App(slice 64 64), Store64, App(const 8), App(add), Store64 *)                
-      (* repeat (step_symex; cbn [fst snd] in * ). *)
-      (* { repeat (eauto || econstructor). }  (* slice 0 64 *)                                        
-      { repeat (eauto || econstructor). }  (* slice 64 64 *)
-      rename x0 into addr_val.
-      (* First Store64: low 8 bytes at addr *)                                                            
-      assert (Haddr2 : eval s2 addr addr_val) by (eapply Hls2; eapply Hls1; exact H2).
-      eapply Store64_R with (v' := Z.land v (Z.ones 64)) (va := addr_val) in HSx;                                         
-      try eassumption; eauto with nocore;                                                                              
-      try solve [rewrite ?Z.shiftr_0_r in *; bitblast.Z.bitblast].
-      destruct_head'_ex; destruct_head'_and. rename x0 into m1. rewrite H3, E0. simpl.
-
-      (* Step through App(const 8), App(add) to learn about addr_hi *)
-      eapply App_R in HSeight as (Hs4 & Hsub4 & Heval_eight).
-      2: { exact H5. }                                                                                                   
-      2: { econstructor; [constructor | reflexivity]. }
-                                                                                                     
-      eapply App_R in HSaddr_hi as (Hs5 & Hsub5 & Heval_addr_hi).                                                
-      2: { exact Hs4. }                                                                                                  
-      2: { eapply ENod with (args' := [addr_val; 8%Z]).                                                                        
-          - constructor; [eapply Hsub4; eapply H6; exact Haddr2 | constructor; [exact Heval_eight | constructor]].
-          - cbn [interp_op]. reflexivity.
-      }
-      cbn [fold_right] in Heval_addr_hi. simpl in Heval_addr_hi.
-      eapply Store64_R with (v' := Z.shiftr v 64) (va := Z.land (addr_val + 8) (Z.ones 64)) in H;
-        try eassumption; eauto with nocore;                                                                              
-        try solve [bitblast.Z.bitblast].
-      destruct_head'_ex; destruct_head'_and. rename x0 into m2.
-      
-      (* Now the main lemma, composition of the two memory operations *)
-      eexists; split.
-      2: { split. eassumption. clear - H1 Hls1 Hls2 H6 Hsub4 Hsub5 H10. eauto 8 using subsumed_trans. }
-      rewrite (SetMem_addr_mod _ (addr_val + 8)) in H.                            
-      eapply (SetMem_compose m addr_val 8 8 v m1 m2).
-      { exact H4. }
-      { exact H. } 
-    }                                                                                       
-    { (* 256-bit store *)
-      admit.
+    { (* 64-bit store: direct write *)
+      eapply Store64_R with (v' := v) in H;
+        try eassumption; eauto with nocore;
+        try solve [rewrite Hbound_old; bitblast.Z.bitblast].
+      destruct H as (m' & Hset & HR' & Hsub'). replace (N.to_nat (64 / 8)) with 8%nat; [|eauto].
+      rewrite Hset.
+      replace (N.to_nat (64 / 8)) with 8%nat by (simpl; lia).
+			eauto 9.
     }
-    { (* err *)
-      step_symex. discriminate H.
-    }
-  Qed. *)
+  }
+  { (* 128-bit case *)
+    eapply R_Store128_of_idx in H; try eassumption; try lia.
+    (* need eval s0 i v — propagate through subsumed *)
+    destruct H as (m' & Hset & HR' & Hsub').
+    exists m'. split; [|split; [exact HR'|solve_subsumed]].
+    rewrite H3, E0. exact Hset.    
+		{ eauto. }
+  }
+  { (* 256-bit case *)
+    eapply R_Store256_of_idx in H; try eassumption; try lia.
+    destruct H as (m' & Hset & HR' & Hsub').
+    exists m'. split; [|split; [exact HR'|solve_subsumed]].
+    rewrite H3, E1. exact Hset.
+    { eauto. }
+  }
+Qed.
 
-
-(* Setting address a to v gives state s' and i evals to v in s *)
-(* then there exists a new machine state m' corresponding to s' s.t. setting a to v in m gives m' *)
-(* note: do the two SetOperand both truncate inputs or not?... *)
 Lemma R_SetOperand {opts : symbolic_options_computed_opt} {descr:description} s m (HR : R s m)
   (sz:OperationSize) (sa:AddressSize) a i _tt s' (H : Symbolic.SetOperand a i s = Success (_tt, s'))
-  v (Hv : eval s i v)
+  v (Hv : eval s i v) (Hsa : sa = 64%N)
   : exists m', SetOperand sa sz m a v = Some m' /\ R s' m' /\ s :< s'.
-Proof using Type.
-Admitted.
-  (* destruct a; cbn in H.                                                                                            
-    - (* reg *) unfold SetReg in H.           
-      destruct ((reg_offset r =? 0)%N && (reg_size r =? widest_reg_size_of r)%N)%bool eqn:Hb.
-      + (* full *) apply andb_prop in Hb. destruct Hb. apply N.eqb_eq in H0, H1. 
-        eapply R_SetReg_full; eauto.
-        unfold SetReg, index_and_shift_and_bitcount_of_reg. rewrite H0, H1, N.eqb_refl, N.eqb_refl. simpl. 
-        rewrite <- H1. exact H.
-      + (* partial *) eapply R_SetReg_partial; eauto.
-        unfold SetReg, index_and_shift_and_bitcount_of_reg. rewrite Hb. exact H.
-    - (* mem *) eapply R_SetMem; eauto.                                                                              
-    - (* const *) cbn in H; inversion H.
-    - cbv [err] in H. discriminate H.
-Qed.  *)
+Proof. 
+	destruct a.
+	{ unfold Symbolic.SetOperand in H. unfold SetOperand. eapply R_SetReg; eauto. }
+	{ unfold Symbolic.SetOperand in H. unfold SetOperand. eapply R_Store; eauto. }
+	{ unfold Symbolic.SetOperand in H. discriminate H. }
+	{ unfold Symbolic.SetOperand in H. discriminate H. }
+Qed. 
+	
 
 Ltac step_SetOperand :=
   match goal with
@@ -1459,47 +1779,6 @@ Ltac step_SetOperand :=
         as (m&?Hm&HR&Hl); clear H
   end.
 
-Lemma acc_range_preserved : forall (acc_val lane_res lane_width : Z) (lane_idx : nat),
-      lane_width > 0 ->
-      Z.shiftr acc_val (Z.of_nat lane_idx * lane_width) = 0 ->
-      let new_acc_val := Z.lor
-          (Z.shiftl (Z.land lane_res (Z.ones lane_width)) (Z.of_nat lane_idx * lane_width))
-          (Z.ldiff acc_val (Z.shiftl (Z.ones lane_width) (Z.of_nat lane_idx * lane_width)))
-      in
-      Z.shiftr new_acc_val (Z.of_nat (S lane_idx) * lane_width) = 0.
-  Proof.
-		intros. 
-	apply Z.bits_inj_iff'; intros i Hi.
-  rewrite Z.shiftr_spec by lia.
-  rewrite Z.bits_0. subst new_acc_val.
-  rewrite Z.lor_spec.
-  (* Show both parts of the lor are 0 at position (S lane_idx) * lane_width + i *)
-  rewrite Z.shiftl_spec by lia.
-  rewrite Z.ldiff_spec.
-  (* The inserted lane occupies [lane_idx * lw, (lane_idx+1) * lw) *)
-  (* Position we're checking: (S lane_idx) * lw + i = (lane_idx + 1) * lw + i *)
-  (* This is >= (lane_idx + 1) * lw, so above the inserted lane *)
-  assert (Hins : Z.testbit (Z.land lane_res (Z.ones lane_width))
-                 (i + Z.of_nat (S lane_idx) * lane_width - Z.of_nat lane_idx * lane_width) = false).
-  { rewrite Z.land_spec, Z.testbit_ones_nonneg by lia.
-    destruct (_ <? _) eqn:E. 
-    apply Z.ltb_lt in E. lia. rewrite Bool.andb_false_r. reflexivity. }
-  rewrite Hins. 
-  (* Now show acc_val bit is 0 *)
-  assert (Hacc_bit : Z.testbit acc_val (Z.of_nat (S lane_idx) * lane_width + i) = false).
-  { 
-	set (lo := Z.of_nat lane_idx * lane_width) in *.
-  replace (Z.of_nat (S lane_idx) * lane_width + i) with (lane_width + i + lo) by (unfold lo; lia).
-  rewrite <- (Z.shiftr_spec acc_val lo (lane_width + i)) by lia.
-  rewrite H0, Z.bits_0. reflexivity.
-	}
-	rewrite Bool.orb_false_l.
-	replace (i + Z.of_nat (S lane_idx) * lane_width) with (Z.of_nat (S lane_idx) * lane_width + i) by lia.
-  rewrite Hacc_bit. reflexivity.
-Qed.
-
-
-
 
 (* === Correspondence lemmas for SymbolicVector general helpers. ===
    Each lemma links a [Symbolic.*] step with its [SemanticVector.*] counterpart.
@@ -1509,18 +1788,18 @@ Section SymbolicVectorProofs.
   Lemma extract_lane_R {opts : symbolic_options_computed_opt} {descr : description}
     s m (HR : R s m)
     (i : idx) (v : Z) (Hv : eval s i v)
-    (lane_idx : nat) (lane_width : Z) (Hlw : (lane_width > 0)%Z)
+    (lane_idx : nat) (lane_width : N) (Hlw : (lane_width > 0)%N)
     res s'
     (H : SymbolicVector.extract_lane i lane_idx lane_width s = Success (res, s'))
     : R s' m /\ s :< s' /\
-      eval s' res (SemanticVector.extract_lane v lane_idx lane_width).
+      eval s' res (SemanticVector.extract_lane v lane_idx (Z.of_N lane_width)).
   Proof using Type.
     unfold SymbolicVector.extract_lane, SemanticVector.extract_lane in *. 
     eapply (App_R s m) in H as (HR' & Hsubs & Heval_res).
     2: { exact HR. }
     2: { repeat (econstructor; eauto). }
     split; [exact HR' | split; [solve_subsumed| ]].
-    repeat rewrite Z2N.id in Heval_res by lia.
+    replace (Z.of_N (N.of_nat lane_idx * lane_width)) with (Z.of_nat lane_idx * Z.of_N lane_width) in Heval_res by lia.
     exact Heval_res.
   Qed.
 
@@ -1531,12 +1810,12 @@ Section SymbolicVectorProofs.
     (Hv1 : eval s i1 v1) (Hv2 : eval s i2 v2)
     (lane_op : op) (binop : Z -> Z -> Z)
     (Hop : interprets_as_binop lane_op binop)
-    (lane_idx : nat) (lane_width : Z) (Hlw : (lane_width > 0)%Z)
+    (lane_idx : nat) (lane_width : N) (Hlw : (lane_width > 0)%N)
     res s'
     (H : SymbolicVector.make_lane i1 i2 lane_op lane_idx lane_width s
         = Success (res, s'))
     : R s' m /\ s :< s' /\
-      eval s' res (SemanticVector.make_lane v1 v2 binop lane_idx lane_width).
+      eval s' res (SemanticVector.make_lane v1 v2 binop lane_idx (Z.of_N lane_width)).
   Proof using Type. 
     unfold SymbolicVector.make_lane, SemanticVector.make_lane in *. repeat step_symex; cbv [fst snd] in *. 
     eapply extract_lane_R in HSl1 as (HR1 & Hsubs1 & Heval_lane1); try eassumption.
@@ -1575,27 +1854,29 @@ Section SymbolicVectorProofs.
     s m (HR : R s m)
     (acc lane : idx) (acc_val lane_val : Z)
     (Hacc : eval s acc acc_val) (Hlane : eval s lane lane_val)
-    (lane_idx : nat) (lane_width : Z) (Hlw : (lane_width > 0)%Z)
+    (lane_idx : nat) (lane_width : N) (Hlw : (lane_width > 0)%N)
     res s'
     (H : SymbolicVector.insert_lane acc lane lane_idx lane_width s
         = Success (res, s'))
     : R s' m /\ s :< s' /\
       eval s' res
-        (Z.lor (SemanticVector.insert_lane lane_val lane_idx lane_width)
+        (Z.lor (SemanticVector.insert_lane lane_val lane_idx (Z.of_N lane_width))
               (Z.ldiff acc_val
-                  (Z.shiftl (Z.ones lane_width)
-                            (Z.of_nat lane_idx * lane_width)))).
+                  (Z.shiftl (Z.ones (Z.of_N lane_width))
+                            (Z.of_nat lane_idx * Z.of_N lane_width)))).
   Proof using Type. 
     cbv [SymbolicVector.insert_lane SemanticVector.insert_lane] in *. 
     eapply (App_R s m) in H as (HR' & Hsubs' & Heval_res). 
-    split; [|split]; try eauto. exact HR. repeat (eauto || econstructor); cbn [interp_op]; repeat rewrite Z2N.id by nia; reflexivity.
+    split; [|split]; try eauto. exact HR. repeat (eauto || econstructor). cbn [interp_op]. 
+    replace (Z.of_N (N.of_nat lane_idx * lane_width)) with (Z.of_nat lane_idx * Z.of_N lane_width) by lia.
+    reflexivity.
   Qed.
 
   (* inductive case of vector_binop_aux_R *)
   Lemma vector_binop_aux_S_lane_idx
     {opts : symbolic_options_computed_opt} {descr : description}
     (i1 i2 : idx) (lane_op : op)
-    (lane_idx n : nat) (lane_width : Z) (acc : idx) s res s'
+    (lane_idx n : nat) (lane_width : N) (acc : idx) s res s'
     (H : SymbolicVector.vector_binop_aux i1 i2 lane_op lane_idx (S n)
           lane_width acc s = Success (res, s'))
     : exists lane_val new_acc s1 s2,
@@ -1609,6 +1890,45 @@ Section SymbolicVectorProofs.
     exists lane_val, new_acc, s0, s1. split; [| split]; eassumption.
   Qed.
 
+  Lemma acc_range_preserved : forall (acc_val lane_res lane_width : Z) (lane_idx : nat),
+    lane_width > 0 ->
+    Z.shiftr acc_val (Z.of_nat lane_idx * lane_width) = 0 ->
+    let new_acc_val := Z.lor
+        (Z.shiftl (Z.land lane_res (Z.ones lane_width)) (Z.of_nat lane_idx * lane_width))
+        (Z.ldiff acc_val (Z.shiftl (Z.ones lane_width) (Z.of_nat lane_idx * lane_width)))
+    in
+    Z.shiftr new_acc_val (Z.of_nat (S lane_idx) * lane_width) = 0.
+  Proof.
+      intros. 
+    apply Z.bits_inj_iff'; intros i Hi.
+    rewrite Z.shiftr_spec by lia.
+    rewrite Z.bits_0. subst new_acc_val.
+    rewrite Z.lor_spec.
+    (* Show both parts of the lor are 0 at position (S lane_idx) * lane_width + i *)
+    rewrite Z.shiftl_spec by lia.
+    rewrite Z.ldiff_spec.
+    (* The inserted lane occupies [lane_idx * lw, (lane_idx+1) * lw) *)
+    (* Position we're checking: (S lane_idx) * lw + i = (lane_idx + 1) * lw + i *)
+    (* This is >= (lane_idx + 1) * lw, so above the inserted lane *)
+    assert (Hins : Z.testbit (Z.land lane_res (Z.ones lane_width))
+                  (i + Z.of_nat (S lane_idx) * lane_width - Z.of_nat lane_idx * lane_width) = false).
+    { rewrite Z.land_spec, Z.testbit_ones_nonneg by lia.
+      destruct (_ <? _) eqn:E. 
+      apply Z.ltb_lt in E. lia. rewrite Bool.andb_false_r. reflexivity. }
+    rewrite Hins. 
+    (* Now show acc_val bit is 0 *)
+    assert (Hacc_bit : Z.testbit acc_val (Z.of_nat (S lane_idx) * lane_width + i) = false).
+    { 
+    set (lo := Z.of_nat lane_idx * lane_width) in *.
+    replace (Z.of_nat (S lane_idx) * lane_width + i) with (lane_width + i + lo) by (unfold lo; lia).
+    rewrite <- (Z.shiftr_spec acc_val lo (lane_width + i)) by lia.
+    rewrite H0, Z.bits_0. reflexivity.
+    }
+    rewrite Bool.orb_false_l.
+    replace (i + Z.of_nat (S lane_idx) * lane_width) with (Z.of_nat (S lane_idx) * lane_width + i) by lia.
+    rewrite Hacc_bit. reflexivity.
+  Qed.
+
   (* Iterates [num_remaining] lanes starting at [lane_idx], folding each into [acc]. *)
   Lemma vector_binop_aux_R {opts : symbolic_options_computed_opt} {descr : description}
         s m (HR : R s m)
@@ -1617,9 +1937,9 @@ Section SymbolicVectorProofs.
         (lane_op : op) (binop : Z -> Z -> Z)
         (Hop : interprets_as_binop lane_op binop)
         (lane_idx num_remaining : nat)
-        (lane_width : Z) (Hlw : (lane_width > 0)%Z)
+        (lane_width : N) (Hlw : (lane_width > 0)%N)
         (acc : idx) (acc_val : Z) (Hacc : eval s acc acc_val)
-        (Hacc_hi : Z.shiftr acc_val (Z.of_nat lane_idx * lane_width) = 0)
+        (Hacc_hi : Z.shiftr acc_val (Z.of_nat lane_idx * Z.of_N lane_width) = 0)
         res s'
         (H : SymbolicVector.vector_binop_aux i1 i2 lane_op lane_idx num_remaining
                                               lane_width acc s
@@ -1627,7 +1947,7 @@ Section SymbolicVectorProofs.
     : R s' m /\ s :< s' /\
       eval s' res
         (Z.lor acc_val
-          (SemanticVector.vector_binop_aux v1 v2 binop lane_idx num_remaining lane_width)).
+          (SemanticVector.vector_binop_aux v1 v2 binop lane_idx num_remaining (Z.of_N lane_width))).
   Proof using Type.
     revert lane_idx s HR acc acc_val Hacc Hacc_hi res s' H Hv1 Hv2; induction num_remaining as [|n IH]; intros.
     { cbv [SemanticVector.vector_binop_aux SymbolicVector.vector_binop_aux] in *. 
@@ -1651,20 +1971,19 @@ Section SymbolicVectorProofs.
     }
   Qed.
     
-
   Lemma SymexVectorBinOp_R {opts : symbolic_options_computed_opt} {descr : description}
     s m (HR : R s m)
     (s_op : OperationSize) (sa : AddressSize) (Hsa : sa = 64%N)
     (dst src1 src2 : ARG)
     (lane_op : op) (binop : Z -> Z -> Z)
     (Hop : interprets_as_binop lane_op binop)
-    (lane_width : Z) (Hlw : (lane_width > 0)%Z)
+    (lane_width : N) (Hlw : (lane_width > 0)%N)
     _tt s'
     (H : @SymbolicVector.SymexVectorBinOp _ _ s_op sa dst src1 src2 lane_op lane_width s
         = Success (_tt, s'))
     : exists m',
         SemanticVector.DenoteVectorBinOp sa s_op m dst src1 src2 binop
-          (N.to_nat (s_op / Z.to_N lane_width)%N) lane_width = Some m'
+          (N.to_nat (s_op / lane_width)%N) (Z.of_N lane_width) = Some m'
         /\ R s' m' /\ s :< s'.
   Proof using Type.
     cbv [SymbolicVector.SymexVectorBinOp] in H. repeat step_symex. cbv [fst snd] in *.
@@ -1675,14 +1994,71 @@ Section SymbolicVectorProofs.
     
     eapply App_R in HSacc as (HR2 & Hsubs2 & Heval_acc); try eauto. 2: repeat econstructor.
     eapply vector_binop_aux_R in HSresult as (HR3 & Hsubs3 & Heval_res); eauto. rewrite Z.lor_0_l in Heval_res. 
-    step_SetOperand.
+    step_SetOperand. exact Hsa.
     eexists. split; [|split]. 
     { cbv [SemanticVector.DenoteVectorBinOp Crypto.Util.Option.bind].
-      rewrite Hdenote1, Hdenote2. exact Hm0. 
-    }
+      rewrite Hdenote1, Hdenote2. exact Hm0. }
     { exact Hs'. }
     { solve_subsumed. }
   Qed.
+
+  Lemma mapM_fold_left_R {A} {opts : symbolic_options_computed_opt} {descr : description}
+  (f_sym : A -> M unit)
+  (f_sem : machine_state -> A -> machine_state)
+  (Hstep : forall a s m s',
+    R s m -> f_sym a s = Success (tt, s') ->
+    R s' (f_sem m a) /\ s :< s')
+  : forall l s m s',
+    R s m ->
+    Symbolic.mapM_ f_sym l s = Success (tt, s') ->
+    R s' (fold_left f_sem l m) /\ s :< s'.
+  Proof using Type.
+    induction l as [|a l IH]; intros s0 m0 s_final HR0 Hsym.
+    - cbv [Symbolic.mapM_ Symbolic.mapM] in Hsym.
+			step_symex; cbv [fst snd] in *; unfold ret in *.
+ 			inversion_ErrorT; Prod.inversion_prod; subst.
+
+      cbn [fold_left]. split; [exact HR0 | solve_subsumed].
+    - cbn [fold_left].
+      cbv [Symbolic.mapM_] in Hsym.
+			step_symex.
+      cbn [Symbolic.mapM] in HSx.
+			repeat step_symex; cbv [fst snd] in *.
+			cbv [ret] in HSx, Hsym.
+ 			inversion_ErrorT; Prod.inversion_prod; subst.
+			destruct b. 
+			edestruct (Hstep _ _ _ _ HR0 HSb) as [HR1 Hsub1].
+			assert (HSbs' : mapM_ f_sym l s1 = Success (tt, s_final)).
+			{ cbv [mapM_ bind ret]. rewrite HSbs. reflexivity. }
+			edestruct (IH _ _ _ HR1 HSbs') as [HR2 Hsub2].
+			split; [exact HR2 | solve_subsumed].
+Qed.
+
+  Lemma vzeroupper_step_R {opts : symbolic_options_computed_opt} {descr : description}
+    (yr : VREG) (s : symbolic_state) (m : machine_state) (s' : symbolic_state)
+    (HR : R s m)
+    (H : (v <- GetReg (VReg yr);
+          lo <- Symbolic.App (slice 0 128, [v]);
+          SetReg (VReg yr) lo)%x86symex s = Success (tt, s'))
+  : R s' (update_reg_with m
+            (fun rs => set_reg rs (VReg yr)
+                          (Z.land (get_reg m (VReg yr)) (Z.ones 128))))
+    /\ s :< s'.
+  Proof using Type.
+    repeat step_symex. step_GetReg. step_App; cbv [fst snd] in *. 
+		{ repeat (econstructor; eauto). }
+		eapply R_SetReg in H; eauto.
+		destruct H as (m' & Hm' & HR' & Hsub'). 
+		Option.inversion_option. subst.
+  	split; [exact HR' | solve_subsumed].
+Qed.
+	
+
+  Lemma interprets_as_add s : interprets_as_binop (add s) (fun a b => Z.land (a + b) (Z.ones (Z.of_N s))).
+    Proof. intros a b. cbn [interp_op fold_right]. rewrite Z.add_0_r. reflexivity. Qed.
+
+  Lemma interprets_as_sub s : interprets_as_binop (sub s) (fun a b => Z.land (a - b) (Z.ones (Z.of_N s))).
+    Proof. intros a b. cbn [interp_op fold_right].  reflexivity. Qed.
 
 End SymbolicVectorProofs.
 
@@ -1933,54 +2309,66 @@ Ltac step :=
 Ltac step1 := step; (eassumption||trivial); [].
 Ltac step01 := solve [step] || step1.
 
-Lemma shiftl_0_r_N (v : Z) : Z.shiftl v (Z.of_N 0) = v.
-Proof. rewrite Z.shiftl_0_r. reflexivity. Qed.
-Print Z.shiftl_0_r.
 
+Lemma set_reg_get_reg (rs : reg_state) (r : REG) :
+  set_reg rs r (get_reg rs r) = rs.
+Proof.
+  cbv [set_reg get_reg].
+  destruct (index_and_shift_and_bitcount_of_reg r) as [[idx shift] bc].
+  apply Tuple.to_list_ext.
+  unshelve erewrite Tuple.from_list_default_eq, Tuple.to_list_from_list.
+  { rewrite ListUtil.length_update_nth. apply Tuple.length_to_list. }
+  apply List.nth_error_ext. intro i.
+  rewrite ListUtil.nth_update_nth.
+  destruct_one_match; trivial.
+  destruct (List.nth_error _ _) eqn:E; trivial. cbn [option_map].
+  f_equal. 
+	subst i.
+replace (Tuple.nth_default 0 (N.to_nat idx) rs) with z.
+2: { rewrite <- Tuple.nth_default_to_list.
+     cbv [nth_default]. rewrite E. reflexivity. }
+cbv [bits_set_slice]. bitblast.Z.bitblast.
+Qed.
+
+Lemma set_mem_get_mem (m : mem_state) addr n v :
+  get_mem m addr n = Some v -> set_mem m addr n v = Some m.
+Proof.
+  cbv [get_mem set_mem Crypto.Util.Option.bind].
+  destruct (load_bytes m (word.of_Z addr) n) as [bs|] eqn:Hl; [|discriminate].
+  intro H. step. subst v. 
+  pose proof (length_load_bytes _ _ _ _ Hl) as Hlen.
+  rewrite <- Hlen, split_le_combine.
+  cbv [store_bytes]. rewrite Hlen, Hl. f_equal.
+  cbv [unchecked_store_bytes].
+  apply map.map_ext. intro k.
+  rewrite Properties.map.get_putmany_dec.
+  rewrite OfListWord.map.get_of_list_word_at.
+  destruct (List.nth_error bs _) eqn:Enth; [|reflexivity].
+  assert (Hi : (Z.to_nat (word.unsigned (word.sub k (word.of_Z addr))) < n)%nat).
+  { rewrite <- Hlen. apply List.nth_error_Some. congruence. }
+  pose proof (Memory.nth_error_load_bytes _ _ _ _ Hl _ Hi) as Hm.
+  rewrite Enth in Hm. rewrite Hm. f_equal.
+  rewrite Z2Nat.id by apply word.unsigned_range.
+  rewrite word.of_Z_unsigned. ring.
+Qed.
 
 (* Denote gets the value of a register, Set actually changes the machine state *)
 (* This says that setting something to its current value returns the same machine state *)
 Lemma SetOperand_same (n : N) (a : ARG) (v : Z) (m m' : machine_state) 
   (Hd : DenoteOperand 64 n m a = Some v) (Hs : SetOperand 64 n m a v = Some m')
   : m = m'.
-Proof using Type.
-Admitted.
-  (* destruct a, m; cbn -[DenoteAddress] in *; repeat (subst; Option.inversion_option).
-  { cbv [update_reg_with set_reg]; cbn in *; f_equal.
-    eapply Tuple.to_list_ext.
-    rewrite <-Tuple.nth_default_to_list in Hd; rewrite <-Hd; clear Hd.
-    unshelve erewrite Tuple.from_list_default_eq, Tuple.to_list_from_list.
-    { abstract (rewrite Crypto.Util.ListUtil.length_update_nth; eapply Tuple.length_to_list). }
-    eapply List.nth_error_ext; intro i; cbv [nth_default].
-    rewrite Crypto.Util.ListUtil.nth_update_nth; destruct_one_match; subst; trivial.
-    destruct_one_match; cbn; trivial; eapply f_equal.
-    eapply Z.bits_inj_iff'; intros i Hi.
-    repeat rewrite ?Z.land_spec, ?Z.ldiff_spec, ?Z.lor_spec, ?bitblast.Z.shiftr_spec', ?bitblast.Z.shiftl_spec', ?Z.testbit_ones, ?Z.testbit_0_l by (clear;lia).
-    destr (i <? 0); cbn; try lia.
-    destr (i - Z.of_N (reg_offset r) <? 0); cbn; try lia.
-    { destr (0 <=? i - Z.of_N (reg_offset r)); cbn; rewrite ?Bool.andb_true_r; trivial.
-      destr (i - Z.of_N (reg_offset r) <? Z.of_N (reg_size r)); cbn; try Btauto.btauto.
-      lia. }
-    destr (0 <=? i - Z.of_N (reg_offset r)); try lia; cbn.
-    replace (i - Z.of_N (reg_offset r) + Z.of_N (reg_offset r)) with i by lia.
-    destr (i - Z.of_N (reg_offset r) <? Z.of_N (reg_size r)); Btauto.btauto. }
-  { destruct m'; cbv [SetMem update_mem_with Crypto.Util.Option.bind get_mem option_map set_mem store_bytes unchecked_store_bytes] in *; repeat (destruct_one_match_hyp || Option.inversion_option).
-    inversion Hs; clear Hs; subst; f_equal.
-    clear E0.
-    change (@map.putmany ?K ?V ?M ?m) with (@map.putmany K V M machine_mem_state).
-    set (word.of_Z _) as a in *; clearbody a.
-    rename n into n'; set (N.to_nat (operand_size m0 n' / 8)) as n in *; clearbody n; clear n'.
-    epose proof (length_load_bytes _ _ _ _ E1) as Hl; rewrite <-Hl, split_le_combine.
-    eapply (@map.map_ext _ _ mem_state _); intro k.
-    rewrite Properties.map.get_putmany_dec, OfListWord.map.get_of_list_word_at.
-    destruct_one_match; trivial.
-    epose proof ListUtil.nth_error_value_length _ _ _ _ E.
-    rewrite <-E; clear E.
-    rewrite (nth_error_load_bytes _ _ _ _ E1 (Z.to_nat (word.unsigned (word.sub k a))) ltac:(lia)).
-    rewrite Z2Nat.id, word.of_Z_unsigned by (eapply Properties.word.unsigned_range).
-    f_equal. ring. }
-Qed. *)
-
+Proof.
+  destruct a; unfold DenoteOperand, SetOperand in *; try discriminate.
+  - (* reg *)
+    repeat Option.inversion_option. subst v m'. unfold update_reg_with.
+    rewrite set_reg_get_reg.
+    destruct m; reflexivity.
+  - (* mem *)
+    cbv [SetMem Crypto.Util.Option.bind] in Hs.
+    apply set_mem_get_mem in Hd.
+    rewrite Hd in Hs.
+    inversion Hs. destruct m; reflexivity.
+Qed.
 
 (* Executing instruction in state s gives state s' *)
 (* exists a machine state correponding to s' s.t.  *)
@@ -2244,22 +2632,20 @@ Proof using Type.
 
   Unshelve. all : match goal with H : context[Syntax.vzeroupper] |- _ => idtac | _ => shelve end; shelve_unifiable.  
   { (* vzeroupper: each YMM gets slice 0 128, matching Z.land _ (Z.ones 128) *)
-    admit.
-  }  
+    eapply mapM_fold_left_R in H. exact H. intros. apply vzeroupper_step_R; assumption. exact HR.
+  }
 
   (* vpaddq *)
   Unshelve. all : match goal with H : context[Syntax.vpaddq] |- _ => idtac | _ => shelve end; shelve_unifiable.
-  { eexists. split. 
-      cbv [SemanticVector.DenoteVectorBinOp Crypto.Util.Option.bind]. rewrite Hv, Hv0.
-      replace (Z.of_N 64) with 64 in Hm0 by lia.
-      erewrite <- interp_vector_binop_eq_vector_binop_values; try lia. 
-      exact Hm0. 
-      split. exact Hs'. eauto.
+  { eapply SymexVectorBinOp_R with
+      (sa := 64%N) (lane_width := 64%N) (lane_op := add 64%N)
+      (binop := fun a b => Z.land (a + b) (Z.ones 64))
+      in H; try (eassumption || lia).
+    apply interprets_as_add.
   }
 
   Unshelve. all: shelve_unifiable.
 	(* cbn. repeat rewrite Z.land_same_r. autorewrite with zsimplify push_Zshift. clear.  cbn.  *)
-  Admitted.
 	
   all: fail_if_goals_remain ().
 (* Qed here hangs until the kernel crashes. Admitting until it can be sped up *)
